nits

examples/steel/OWGCounterInv.fst
@@ -41,57 +41,36 @@ module A = Steel.Effect.Atomic
 
 open Steel.DisposableInvariant
 
-#set-options "--using_facts_from '* -FStar.Tactics -FStar.Reflection' --fuel 0 --ifuel 0"
+#set-options "--using_facts_from '* -FStar.Tactics -FStar.Reflection' --fuel 0 --ifuel 0 --ide_id_info_off"
 
-let half_perm = half_perm (MkPerm FStar.Real.one)
-
-let fst = fst
-let snd = snd
+//let half_perm = half_perm (MkPerm FStar.Real.one)
 
 (**** A few wrappers over library functions ****)
 
-(*
- * Wrapper over ghost_gather that rewrites sum_perm half_perm half_perm to full_perm
- *)
-
-#set-options "--print_implicits"
-
 let ghost_gather (#uses:inames) (v1 #v2:G.erased int) (r:ghost_ref int)
   : SteelAtomic unit uses unobservable
-      (ghost_pts_to r half_perm v1 `star`
-       ghost_pts_to r half_perm v2)
+      (ghost_pts_to r (P.half_perm full_perm) v1 `star`
+       ghost_pts_to r (P.half_perm full_perm) v2)
       (fun _ -> ghost_pts_to r full_perm v1)
       (fun _ -> True)
       (fun _ _ _ -> v1 == v2)
   = ghost_gather #_ #_ #_ #_ #v1 #v2 r;
     ()
 
-(*
- * Similar wrapper over ghost_share that rewrites (half_perm full_perm) to half_perm
- *)
 let ghost_share (#uses:inames) (v1 #v2:G.erased int) (r:ghost_ref int)
   : SteelAtomic unit uses unobservable
       (ghost_pts_to r full_perm v1)
-      (fun _ -> ghost_pts_to r half_perm v1 `star`
-             ghost_pts_to r half_perm v2)
+      (fun _ -> ghost_pts_to r (P.half_perm full_perm) v1 `star`
+             ghost_pts_to r (P.half_perm full_perm) v2)
       (fun _ -> v1 == v2)
       (fun _ _ _ -> True)
   = ghost_share #_ #_ #_ #v1 r; ()
 
-(*
- * Perm rewriting wrappers over share and gather invariant
- *)
-let share_invariant (#p:slprop) (#uses:inames) (i:inv p)
-  : SteelAtomicT unit uses unobservable
-      (active full_perm i)
-      (fun _ -> active half_perm i `star` active half_perm i)
-  = share i
-
 let gather_invariant (#p:slprop) (#uses:inames) (i:inv p)
   : SteelAtomicT unit uses unobservable
-      (active half_perm i `star` active half_perm i)
+      (active (P.half_perm full_perm) i `star` active (P.half_perm full_perm) i)
       (fun _ -> active full_perm i)
-  = gather #_ #half_perm #half_perm #_ i; ()
+  = gather #_ #(P.half_perm full_perm) #(P.half_perm full_perm) #_ i; ()
 
 (*
  * A SteelAtomic to Steel lift for with_invariant
@@ -123,8 +102,8 @@ let with_invariant (#a:Type)
 [@@ __reduce__]
 let inv_pred (r:ref int) (r1 r2:ghost_ref int) =
   fun (w:G.erased int & G.erased int) ->
-    ghost_pts_to r1 half_perm (fst w) `star`
-    ghost_pts_to r2 half_perm (snd w) `star`
+    ghost_pts_to r1 (P.half_perm full_perm) (fst w) `star`
+    ghost_pts_to r2 (P.half_perm full_perm) (snd w) `star`
     pts_to r full_perm (fst w + snd w)
 
 (*
@@ -147,11 +126,11 @@ let inv_equiv_lemma (r:ref int) (r1 r2:ghost_ref int)
           (ensures interp (inv_slprop r r2 r1) m)
           [SMTPat ()]
       = let w : G.erased (G.erased int & G.erased int) = id_elim_exists (inv_pred r r1 r2) m in
-        assert ((ghost_pts_to r1 half_perm (snd (snd w, fst w)) `star`
-                 ghost_pts_to r2 half_perm (fst (snd w, fst w)) `star`
+        assert ((ghost_pts_to r1 (P.half_perm full_perm) (snd (snd w, fst w)) `star`
+                 ghost_pts_to r2 (P.half_perm full_perm) (fst (snd w, fst w)) `star`
                  pts_to r full_perm (G.hide (G.reveal (fst (snd w, fst w)) + G.reveal (snd (snd w, fst w))))) `equiv`
-                (ghost_pts_to r2 half_perm (fst (snd w, fst w)) `star`
-                 ghost_pts_to r1 half_perm (snd (snd w, fst w)) `star`
+                (ghost_pts_to r2 (P.half_perm full_perm) (fst (snd w, fst w)) `star`
+                 ghost_pts_to r1 (P.half_perm full_perm) (snd (snd w, fst w)) `star`
                  pts_to r full_perm (G.hide (G.reveal (fst (snd w, fst w)) + G.reveal (snd (snd w, fst w)))))) by Steel.Memory.Tactics.canon ();
 
         intro_h_exists (snd w, fst w) (inv_pred r r2 r1) m in
@@ -160,23 +139,6 @@ let inv_equiv_lemma (r:ref int) (r1 r2:ghost_ref int)
 
 
 (**** Helpers for the counter implementation ****)
-
-(*
- * Allocating a disposable invariant that protects inv_slprop
- *)
-let new_inv (#uses:inames) (#v:G.erased int) (r:ref int) (r1 r2:ghost_ref int)
-  : SteelAtomicT (inv (inv_slprop r r1 r2)) uses unobservable
-      (pts_to r full_perm v  `star`
-       ghost_pts_to r1 half_perm 0 `star`
-       ghost_pts_to r2 half_perm v)
-      (fun i -> active full_perm i)
-  = //rewrite the pts_to r in the form expected by inv_slprop
-    change_slprop (pts_to r _ _)
-                  (pts_to r full_perm (G.hide (G.reveal (fst (G.hide 0, v)) + G.reveal (snd (G.hide 0, v)))))
-                  (fun _ -> ());
-    intro_exists (G.hide 0, v) (inv_pred r r1 r2);
-    new_inv (inv_slprop r r1 r2)
-
 let incr (n:G.erased int) = G.elift1 (fun (n:int) -> n + 1) n
 
 (*
@@ -195,15 +157,15 @@ assume val incr_atomic (#uses:inames) (#v:G.erased int) (r:ref int)
  *)
 let incr_ghost_contrib (#uses:inames) (#v1 #v2:G.erased int) (r:ghost_ref int)
   : SteelAtomic unit uses unobservable
-      (ghost_pts_to r half_perm v1 `star`
-       ghost_pts_to r half_perm v2)
-      (fun _ -> ghost_pts_to r half_perm (incr v1) `star`
-             ghost_pts_to r half_perm (incr v2))
+      (ghost_pts_to r (P.half_perm full_perm) v1 `star`
+       ghost_pts_to r (P.half_perm full_perm) v2)
+      (fun _ -> ghost_pts_to r (P.half_perm full_perm) (incr v1) `star`
+             ghost_pts_to r (P.half_perm full_perm) (incr v2))
       (fun _ -> True)
       (fun _ _ _ -> v1 == v2)
-  = ghost_gather v1 #v2 r;
+  = ghost_gather v1 r;
     ghost_write r (incr v1);
-    ghost_share (incr v1) #(incr v2) r
+    ghost_share (incr v1) r
 
 (*
  * Another form of the inv_slprop with conditional on the ghost refs
@@ -226,11 +188,11 @@ let incr_with_inv_slprop
   : SteelAtomicT unit (Set.singleton name) observable
       (inv_slprop_conditional r r_mine r_other b
        `star`
-       ghost_pts_to r_mine half_perm n_ghost)
+       ghost_pts_to r_mine (P.half_perm full_perm) n_ghost)
       (fun _ ->
        inv_slprop_conditional r r_mine r_other b
        `star`
-       ghost_pts_to r_mine half_perm (incr n_ghost))
+       ghost_pts_to r_mine (P.half_perm full_perm) (incr n_ghost))
   = //get inv_slprop in the context
     change_slprop (inv_slprop_conditional _ _ _ _)
                   (inv_slprop _ _ _) (fun _ -> ());
@@ -239,8 +201,6 @@ let incr_with_inv_slprop
     incr_ghost_contrib #_ #n_ghost #(fst w) r_mine;
 
     //restore inv_slprop, by first writing r to a form expected by the invariant
-    change_slprop (pts_to r full_perm _)
-                  (pts_to r full_perm (G.hide (incr (fst w) + snd w))) (fun _ -> ());
     intro_exists (incr (fst w), snd w) (inv_pred r r_mine r_other);
     change_slprop (inv_slprop _ _ _)
                   (inv_slprop_conditional _ _ _ _) (fun _ -> ())
@@ -253,8 +213,8 @@ let incr_with_invariant
   (i:inv (inv_slprop_conditional r r_mine r_other b))
   ()
   : SteelT unit
-      (active half_perm i `star` ghost_pts_to r_mine half_perm n_ghost)
-      (fun _ -> active half_perm i `star` ghost_pts_to r_mine half_perm (incr n_ghost))
+      (active (P.half_perm full_perm) i `star` ghost_pts_to r_mine (P.half_perm full_perm) n_ghost)
+      (fun _ -> active (P.half_perm full_perm) i `star` ghost_pts_to r_mine (P.half_perm full_perm) (incr n_ghost))
   = with_invariant i
       (incr_with_inv_slprop r r_mine r_other n_ghost b (name i))
 
@@ -271,14 +231,16 @@ let incr_main (#v:G.erased int) (r:ref int)
     let r2 = ghost_alloc v in
 
     //split their permissions
-    ghost_share 0 r1;
-    ghost_share v r2;
+    R.ghost_share r1;
+    R.ghost_share r2;
 
     //create the invariant
-    let i = new_inv r r1 r2 in
+
+    intro_exists (G.hide 0, v) (inv_pred r r1 r2);
+    let i = new_inv (inv_slprop r r1 r2) in
 
     //split the invariant permission
-    share_invariant i;
+    share i;
 
     //invoke the two threads
     let _ =
@@ -292,4 +254,4 @@ let incr_main (#v:G.erased int) (r:ref int)
 
     //drop the ghost refs
     ghost_gather (incr 0) r1; drop (ghost_pts_to r1 _ _);
-    ghost_gather (incr v) r2; drop (ghost_pts_to r2 _ _); ()
+    ghost_gather (incr v) r2; drop (ghost_pts_to r2 _ _)
